

ISyE/Math 6759 Stochastic Processes in Finance – I

Homework Set 6

Vidit Pokharna, 903772087

12/01/2025

Problem 1

$$\frac{dS(t)}{S(t)} = 0.05 dt + 0.2 dZ(t), \quad S(0) = 0.5$$

$$S(1) = S(0) \exp\left((\mu - \tfrac{1}{2}\sigma^2) + \sigma Z_1\right), \quad \mu = 0.05, \sigma = 0.2$$

$$E[S(1)^a] = S(0)^a \exp\left(a(\mu - \tfrac{1}{2}\sigma^2) + \tfrac{1}{2}a^2\sigma^2\right) = 1.4$$

$$S(0)^a = 0.5^a, \quad \mu - \tfrac{1}{2}\sigma^2 = 0.05 - 0.5 \cdot 0.2^2 = 0.03, \quad \tfrac{1}{2}\sigma^2 = 0.5 \cdot 0.2^2 = 0.02$$

$$0.5^a \exp(0.03a + 0.02a^2) = 1.4$$

$$a \ln 0.5 + 0.03a + 0.02a^2 = \ln 1.4$$

$$0.02a^2 + (\ln 0.5 + 0.03)a - \ln 1.4 = 0$$

$$a = \frac{-(\ln 0.5 + 0.03) \pm \sqrt{(\ln 0.5 + 0.03)^2 + 0.08 \ln 1.4}}{0.04}$$

$$a_1 \approx -0.4999, \quad a_2 \approx 33.6572, \quad a = a_1 \ (a < 0)$$

Risk-neutral measure:

$$\frac{dS(t)}{S(t)} = r dt + 0.2 dW(t), \quad r = 0.03$$

$$S(1) = S(0) \exp\left((r - \tfrac{1}{2}\sigma^2) + \sigma W_1\right), \quad r - \tfrac{1}{2}\sigma^2 = 0.03 - 0.02 = 0.01$$

$$E^{\mathbb{Q}}[S(1)^a] = S(0)^a \exp\left(a(r - \tfrac{1}{2}\sigma^2) + \tfrac{1}{2}a^2\sigma^2\right) = 0.5^a \exp(0.01a + 0.02a^2)$$

$$E^{\mathbb{Q}}[S(1)^a] \Big|_{a \approx -0.4999} \approx 1.4141$$

$$V_0 = e^{-r} E^{\mathbb{Q}}[S(1)^a] = e^{-0.03} \cdot 0.5^a \exp(0.01a + 0.02a^2)$$

$$V_0 \approx e^{-0.03} \cdot 1.4141 \approx 1.3723$$

Problem 2

(a) By Itô's formula,

$$\begin{aligned} d\Pi(t) &= dF(t, S(t)) \\ &= F_t(t, S(t)) dt + F_s(t, S(t)) dS(t) + \frac{1}{2} F_{ss}(t, S(t)) d\langle S \rangle_t \\ &= \left(F_t + rSF_s + \frac{1}{2} \sigma^2 S^2 F_{ss} \right)(t, S(t)) dt + \sigma S(t) F_s(t, S(t)) dW(t) \end{aligned}$$

Using the PDE,

$$F_t + rSF_s + \frac{1}{2} \sigma^2 S^2 F_{ss} = rF,$$

so

$$d\Pi(t) = rF(t, S(t)) dt + \sigma S(t) F_s(t, S(t)) dW(t) = r\Pi(t) dt + g(t) dW(t),$$

where

$$g(t) = \sigma S(t) F_s(t, S(t))$$

(b)

$$Z(t) = \frac{\Pi(t)}{B(t)}$$

Since $B(t) = e^{rt}$, we have

$$dB(t) = rB(t) dt, \quad d(B(t)^{-1}) = -rB(t)^{-1} dt$$

Using Itô's formula (or product rule) for $Z(t) = \Pi(t)B(t)^{-1}$,

$$\begin{aligned} dZ(t) &= B(t)^{-1} d\Pi(t) + \Pi(t) d(B(t)^{-1}) + d\Pi(t) d(B(t)^{-1}) \\ &= B(t)^{-1} (r\Pi(t) dt + g(t) dW(t)) + \Pi(t) (-rB(t)^{-1} dt), \end{aligned}$$

and the quadratic covariation term vanishes since B^{-1} is deterministic.

Thus

$$dZ(t) = \frac{g(t)}{B(t)} dW(t)$$

And then we know Z is a martingale with dynamics

$$dZ(t) = Z(t) \sigma_Z(t) dW(t),$$

where

$$\sigma_Z(t) = \frac{g(t)}{\Pi(t)} = \frac{\sigma S(t) F_s(t, S(t))}{F(t, S(t))}$$

Problem 3

Payoff at T : $GL(T) = \ln S(T)$

Under the risk-neutral measure \mathbb{Q} ,

$$\frac{dS(t)}{S(t)} = r dt + \sigma dW(t),$$

so for $0 \leq t \leq T$,

$$S(T) = S(t) \exp \left((r - \tfrac{1}{2}\sigma^2)(T - t) + \sigma(W(T) - W(t)) \right)$$

Thus

$$\ln S(T) = \ln S(t) + (r - \tfrac{1}{2}\sigma^2)(T - t) + \sigma(W(T) - W(t))$$

Given \mathcal{F}_t , the increment $W(T) - W(t) \sim N(0, T - t)$ with mean 0, so

$$\mathbb{E}^{\mathbb{Q}}[\ln S(T) \mid \mathcal{F}_t] = \ln S(t) + (r - \tfrac{1}{2}\sigma^2)(T - t)$$

The arbitrage-free price process $\Pi(t)$ of $GL(T)$ is

$$\Pi(t) = B(t) \mathbb{E}^{\mathbb{Q}} \left[\frac{\ln S(T)}{B(T)} \mid \mathcal{F}_t \right] = e^{-r(T-t)} \mathbb{E}^{\mathbb{Q}}[\ln S(T) \mid \mathcal{F}_t]$$

Therefore

$$\boxed{\Pi(t) = e^{-r(T-t)} (\ln S(t) + (r - \tfrac{1}{2}\sigma^2)(T - t))}$$

In particular, at time 0,

$$\Pi(0) = e^{-rT} (\ln S(0) + (r - \tfrac{1}{2}\sigma^2)T)$$

Problem 4

$$\begin{aligned}
\tau &= T - t \\
C(t) &= e^{-r\tau} \mathbb{E}^{\mathbb{Q}}[(S(T) - K)^+ \mid \mathcal{F}_t] \\
S(T) &= S(t) \exp\left((r - \tfrac{1}{2}\sigma^2)\tau + \sigma\sqrt{\tau} Z\right), \quad Z \sim N(0, 1) \\
d_1 &= \frac{\ln \frac{S(t)}{K} + (r + \tfrac{1}{2}\sigma^2)\tau}{\sigma\sqrt{\tau}}, \quad d_2 = d_1 - \sigma\sqrt{\tau} \\
C(t) &= S(t)N(d_1) - Ke^{-r\tau}N(d_2)
\end{aligned}$$

Problem 5

$$\begin{aligned}
X &= S(T)^\beta \\
\ln S(T) &= \ln S(t) + (r - \tfrac{1}{2}\sigma^2)\tau + \sigma\sqrt{\tau} Z, \quad Z \sim N(0, 1) \\
\mathbb{E}^{\mathbb{Q}}[S(T)^\beta \mid \mathcal{F}_t] &= S(t)^\beta \exp\left(\beta(r - \tfrac{1}{2}\sigma^2)\tau + \tfrac{1}{2}\beta^2\sigma^2\tau\right) \\
\Pi(t) &= e^{-r\tau} \mathbb{E}^{\mathbb{Q}}[S(T)^\beta \mid \mathcal{F}_t] = S(t)^\beta \exp\left((\beta - 1)r\tau + \tfrac{1}{2}\beta(\beta - 1)\sigma^2\tau\right)
\end{aligned}$$

Problem 6

$$\begin{aligned}
\tau &= T - t \\
\Pi_6(t) &= e^{-r\tau} K \mathbb{P}^{\mathbb{Q}}(\alpha \leq S(T) \leq \beta \mid \mathcal{F}_t) \\
\ln S(T) &= \ln S(t) + (r - \tfrac{1}{2}\sigma^2)\tau + \sigma\sqrt{\tau} Z, \quad Z \sim N(0, 1) \\
d_\alpha &= \frac{\ln(\alpha/S(t)) - (r - \tfrac{1}{2}\sigma^2)\tau}{\sigma\sqrt{\tau}}, \quad d_\beta = \frac{\ln(\beta/S(t)) - (r - \tfrac{1}{2}\sigma^2)\tau}{\sigma\sqrt{\tau}} \\
\Pi_6(t) &= Ke^{-r\tau}(N(d_\beta) - N(d_\alpha))
\end{aligned}$$

Problem 7

$$\begin{aligned}
X &= \frac{S(T_1)}{S(T_0)} \\
\Pi_7(t) &= e^{-r(T_1-t)} \mathbb{E}^{\mathbb{Q}}\left[\frac{S(T_1)}{S(T_0)} \mid \mathcal{F}_t\right] \\
\Pi_7(t) &= \begin{cases} e^{-r(T_0-t)}, & 0 \leq t \leq T_0, \\ \frac{S(t)}{S(T_0)}, & T_0 < t \leq T_1. \end{cases}
\end{aligned}$$

Problem 8

$$dS_t = \alpha S_t dt + \sigma S_t d\bar{W}_1(t), \quad dY_t = \beta Y_t dt + \delta Y_t d\bar{W}_2(t), \quad \bar{W}_1 \perp \bar{W}_2$$

$$Z_t := S_t Y_t$$

$$dZ_t = S_t dY_t + Y_t dS_t + dS_t dY_t$$

$$dS_t dY_t = \sigma S_t \delta Y_t d\bar{W}_1 d\bar{W}_2 = 0$$

$$dZ_t = (\alpha + \beta) Z_t dt + \sigma Z_t d\bar{W}_1 + \delta Z_t d\bar{W}_2$$

$$\exists \bar{W} : \quad \sigma d\bar{W}_1 + \delta d\bar{W}_2 = v d\bar{W}, \quad v := \sqrt{\sigma^2 + \delta^2}$$

$$\Rightarrow \quad \frac{dZ_t}{Z_t} = (\alpha + \beta) dt + v d\bar{W}_t$$

$$\text{under } \mathbb{Q} : \quad \frac{dZ_t}{Z_t} = r dt + v dW_t$$

$$Z_T = Z_t \exp\left((r - \tfrac{1}{2}v^2)(T - t) + v\sqrt{T - t} Z\right), \quad Z \sim N(0, 1)$$

$$\ln Z_T \sim N(m, v^2(T - t)), \quad m = \ln Z_t + (r - \tfrac{1}{2}v^2)(T - t)$$

$$X = \ln(Z_T^2) = 2 \ln Z_T$$

$$\mathbb{E}^{\mathbb{Q}}[X \mid Z_t = z] = 2 \mathbb{E}^{\mathbb{Q}}[\ln Z_T \mid Z_t = z] = 2\left(\ln z + (r - \tfrac{1}{2}v^2)(T - t)\right)$$

$$\Pi(t, z) = e^{-r(T-t)} \mathbb{E}^{\mathbb{Q}}[X \mid Z_t = z]$$

$$\boxed{\Pi(t, z) = 2e^{-r(T-t)}\left(\ln z + (r - \tfrac{1}{2}(\sigma^2 + \delta^2))(T - t)\right)}$$

Problem 9

$$dS_t = rS_t dt + \sigma S_t dW_t$$

$$V_t = S_t^a$$

$$dV_t = aS_t^{a-1}dS_t + \frac{1}{2}a(a-1)S_t^{a-2}(dS_t)^2$$

$$(dS_t)^2 = \sigma^2 S_t^2 dt$$

$$dV_t = \left(ar + \frac{1}{2}a(a-1)\sigma^2 \right) S_t^a dt + a\sigma S_t^a dW_t$$

$$\text{Choose } a = -\frac{2r}{\sigma^2} : \quad ar + \frac{1}{2}a(a-1)\sigma^2 = r$$

$$\Rightarrow \quad dV_t = rV_t dt + a\sigma V_t dW_t$$

$$V_t = S_t^{-2r/\sigma^2}$$

Problem 10

$$dS_t = \mu S_t dt + \sigma S_t dW_t$$

$$X_t = S_t^n$$

$$dX_t = nS_t^{n-1}dS_t + \frac{1}{2}n(n-1)S_t^{n-2}(dS_t)^2$$

$$(dS_t)^2 = \sigma^2 S_t^2 dt$$

$$dX_t = \left(n\mu + \frac{1}{2}n(n-1)\sigma^2 \right) S_t^n dt + n\sigma S_t^n dW_t$$

$$d(S_t^n) = \mu_n S_t^n dt + \sigma_n S_t^n dW_t, \quad \mu_n = n\mu + \frac{1}{2}n(n-1)\sigma^2, \quad \sigma_n = n\sigma$$